formalization/thesis/Isotope/Elgot/RA.lean
@@ -3,6 +3,7 @@ import Isotope.Elgot.RA.Trace
 import Isotope.Elgot.RA.Rewrite
 import Isotope.Elgot.RA.Closure
 import Isotope.Elgot.RA.Monad
+import Isotope.Elgot.RA.Iteration
 
 /-!
 # A release/acquire trace monad
